specs/lemmas/Spec.Hash.Incremental.fsti
@@ -10,6 +10,7 @@ open FStar.Mul
 open Lib.Sequence
 open Lib.ByteSequence
 open Lib.IntTypes
+module Loops = Lib.LoopCombinators
 
 #reset-options "--fuel 0 --ifuel 0 --z3rlimit 100"
 
@@ -104,6 +105,22 @@ let blake2_hash_incremental
   finish a s
 
 let hash = Spec.Agile.Hash.hash
+
+val repeati_blake2_update1_is_update_multi
+  (a:hash_alg{is_blake a}) (nb prev : nat)
+  (d : bytes)
+  (hash : words_state' a) :
+  Lemma
+  (requires (
+    nb * block_length a <= Seq.length d /\
+    prev + Seq.length d <= Blake2.max_limb (to_blake_alg a) /\
+    prev + nb * block_length a <= max_extra_state a
+  ))
+  (ensures (
+    let blocks, _ = Seq.split d (nb * block_length a) in
+    (Loops.repeati #(words_state' a) nb (Blake2.blake2_update1 (to_blake_alg a) prev d) hash,
+     nat_to_extra_state a (prev + nb * block_length a)) ==
+       update_multi a (hash, nat_to_extra_state a prev) blocks))
 
 val blake2_is_hash_incremental
   (a: hash_alg{is_blake a})
